Very ugly but working proof tree retrieval

PaperProof.lean
@@ -2,99 +2,236 @@ import Mathlib.Data.Nat.Prime
 import Mathlib.Tactic.LibrarySearch
 import Mathlib.Tactic.Linarith
 import Std.Classes.Dvd
-
+import Lean.Elab.Tactic
 import Lean
+import Lean.Environment
+import Lean.Elab.Frontend
+import Lean.Elab.InfoTree
+import Lean.Data.Options
+import Lean.Widget
+
+open Lean
+open Lean Elab
+open Lean Meta
+open Lean.Elab.Tactic
 open Lean Widget
 
-theorem infinitude_of_primes : ∀ N, ∃ p, p ≥ N ∧ Nat.Prime p := by
-  intro N
-  
-  let M := Nat.factorial N + 1
-  let p := Nat.minFac M
+def solvedEmoji := "✅"
 
-  use p
-  
-  have pp : Nat.Prime p := by {
-    have minFac_prime := @Nat.minFac_prime M
-    apply minFac_prime
-    have := Nat.factorial_pos N
-    linarith
-  }
-  have ppos: p ≥ N := by {
-    apply by_contradiction
-    intro pln
-    have h₁ : p ∣ Nat.factorial N := by  {
-      refine pp.dvd_factorial.mpr ?_
-      exact le_of_not_ge pln
-    }
-    have h₂ : p ∣ Nat.factorial N + 1 := by apply Nat.minFac_dvd
-    have sp : {a : Nat} → (p ∣ Nat.factorial N + a) → p ∣ a := (Nat.dvd_add_right h₁).mp
-    have h : p ∣ 1 := sp h₂
-    apply Nat.Prime.not_dvd_one pp h
-  }
-  exact ⟨ ppos, pp ⟩
+def printInfo (info : Info) (printAll : Bool) : MessageData :=
+  match info with
+  | .ofTacticInfo ti => 
+    if ti.stx.prettyPrint.pretty.startsWith "have" then
+      m!"TCTCINFO {ti.stx.prettyPrint}"
+    else
+      if printAll then m!"tactic info ${ti.elaborator} ${info.stx.getPos?}, {info.stx.getTailPos?} <{ti.stx.prettyPrint}>" else m!""
+  | .ofTermInfo i => if printAll then m!"term info {info.stx.prettyPrint}" else m!""
+  | .ofCommandInfo _ => if printAll then m!"command info {info.stx.prettyPrint}" else m!""
+  | .ofMacroExpansionInfo _ => m!"macro expansion info"
+  | .ofFieldInfo _ => m!"field info"
+  | .ofCompletionInfo _ => m!"completion info"
+  | .ofCustomInfo _ => m!"custom info"
+  | _ => if printAll then m!"other info" else m!""
 
-def g : Nat → Nat → Int := fun n m => n + m 
-def f : Nat → Int := g 3
+def goDeeper (info : Info) : Bool :=
+  match info with
+  | .ofTacticInfo i => 
+    if s!"{i.stx.prettyPrint}".startsWith "let" then
+      false
+    else
+      true
+  | _ => true
 
-def my_id (n : Nat) := n
+def isSameSpan (infoTree : InfoTree) (fromPos toPos : String.Pos) : Bool :=
+  match infoTree with
+  | InfoTree.node i _ =>
+    let fromPos' := i.stx.getPos?.get!
+    let toPos' := i.stx.getTailPos?.get!
+    fromPos == fromPos' && toPos == toPos'
+  | _ => false
 
-def functions_example : True := by
-  let y := f 4
-  
-  exact True.intro
+-- should find all term info nodes which have no children
+partial def findSubFrames (infoTree : InfoTree) : List String :=
+  match infoTree with
+  | InfoTree.node i children =>
+    if children.size == 0 then
+      match i with
+      | .ofTermInfo info => [s!"{i.stx.prettyPrint}"]
+      | _ => []
+    else
+      children.map findSubFrames |>.toList.join
+  | _ => []
+
+structure Frame where
+  fromType: String
+  toType: String
+  action: String
+  subFrames : List String
+
+structure TreeState where
+  types : PersistentHashMap String String
+  frames : List Frame
+
+instance : ToString Frame where
+  toString f := s!"from: {f.fromType}, action: {f.action} to: {f.toType} subframes: {f.subFrames}"
+
+abbrev FrameStack T := StateT TreeState IO T
+
+def toStrType (infoTree : InfoTree) (ctx : Option ContextInfo) (lctx : Option LocalContext) : FrameStack String := do
+  if let some ctx := ctx then
+    match infoTree with
+    | InfoTree.node (.ofTermInfo i) _ => ctx.runMetaM (lctx.getD {}) $ do
+      return s!"{← ppExpr i.expr}"
+    | InfoTree.node i _ => return s!"{i.stx.prettyPrint}"
+    | _ => return s!""
+  else return "XXX"
+
+def toStrSyntax (infoTree : InfoTree) : String :=
+  match infoTree with
+  | InfoTree.node i _ => s!"{i.stx.prettyPrint}"
+  | _ => s!""
+
+def addFrame (frame : Frame) : FrameStack Unit :=
+  modify fun state => {state with frames := frame :: state.frames }
+
+def addName (name type : String) : FrameStack Unit :=
+  modify fun state => {state with types := state.types.insert name type }
+
+def isHaveTerm (info : Info) (children: PersistentArray InfoTree): Bool :=
+  match info with
+  | .ofTermInfo i => s!"{i.stx.prettyPrint}".trimLeft.startsWith "let_fun" && children.size == 4
+  | _ => false
+
+def isTactic (names: List String) (info : Info) : Option (String × TacticInfo) := do
+  match info with
+  | .ofTacticInfo i => 
+    for name in names do
+      if s!"{i.elaborator}".trimRight.toLower.endsWith name then
+        return (name, i)
+    none
+  | _ => none
+
+structure Goals where
+  goalsBefore : List MVarId
+  goalsAfter : List MVarId
+  deriving ToJson
+
+partial def getLCtx (info : Info) (children : PersistentArray InfoTree): Option LocalContext :=
+  match info with
+  | .ofTermInfo i => i.lctx
+  | .ofMacroExpansionInfo i => i.lctx
+  | .ofFieldInfo i => i.lctx
+  | .ofTacticInfo i => if children.size > 0 then
+    -- call recursively because for example on `intro N` we had not term above to set the context.
+    match children[0]! with
+      | .node ii cs => getLCtx ii cs
+      | _ => none
+    else none
+  | _ => none
+
+def getType (ctx: Option ContextInfo) (lctx : Option LocalContext) (tInfo: TacticInfo) (before := false) : FrameStack String :=
+  let goals := if before then tInfo.goalsBefore else tInfo.goalsAfter
+  let lctx := lctx.getD {}
+  if let (some context) := (ctx) then
+    if goals.length > 0 then
+      context.runMetaM lctx $ do
+        let mvar := goals[0]!
+        let type ← mvar.getType
+        return s!"{← ppExpr type}"
+    else pure solvedEmoji
+  else pure solvedEmoji
 
 
-def dist (x y : Int): Nat := (x - y).natAbs
-def f'(x : Int): Int := x + 1
+partial def parseTacticProof (ctx : Option ContextInfo) (lctx : Option LocalContext) (infoTree : InfoTree) (name: String := "top level") : FrameStack MessageData := do
+  match infoTree with
+  | InfoTree.node i children =>
+    let lctx := if let some c := getLCtx i children then c else lctx
+    let fromPos := i.stx.getPos?.get!
+    let toPos := i.stx.getTailPos?.get!
 
-theorem limit:
-  ∃ L, ∀ ε, ε > 0 → ∃ N, ∀ n, n ≥ N → dist (f' n) L < ε := by sorry
+    let processTactic (tacticName : String) (tInfo : TacticInfo) : FrameStack MessageData := do
+      let subFrames := children.map (fun c => findSubFrames c) |>.toList.join
+      let type ← getType ctx lctx tInfo
+      let beforeGoal ← getType ctx lctx tInfo true
+      let t := {
+        fromType := beforeGoal,
+        toType := type,
+        action := s!"{i.stx.prettyPrint}",
+        subFrames := subFrames}
+      addFrame t
+      let info := m!"!!!! {tInfo.elaborator} {tacticName} {i.stx.prettyPrint}"
+      let cs := (← children.mapM (parseTacticProof ctx lctx)) |>.toList
+      return MessageData.group $ info ++ MessageData.nest 2 (Format.line ++ MessageData.ofList cs)
 
-theorem using_primes : a → a := by
-  let x := infinitude_of_primes
-  let y := limit 
+    if children.size == 1 && isSameSpan children[0]! fromPos toPos then
+      parseTacticProof ctx lctx children[0]! -- this is helpful only for tree output, not parsing
+    else if children.size == 2 && i.stx.prettyPrint.pretty.trimLeft.startsWith "focus" then
+      parseTacticProof ctx lctx children[1]! -- same as above
+    else if isHaveTerm i children then
+      -- let type := getType ctx lctx i
+      let vals ← children.mapM (fun c => toStrType c ctx lctx)
+      let name := toStrSyntax children[2]!
+      addName name vals[0]!
+      if vals[1]!.trimLeft.startsWith "by" then
+        let info := "BBB" ++ printInfo i true
+        let r ← parseTacticProof ctx lctx children[1]!
+        return info ++ r
+      else
+        let subFrames := findSubFrames children[1]!
+        let t := {fromType := vals[0]!, toType := solvedEmoji, action:= s!"exact {vals[1]!}", subFrames := subFrames}
+        addFrame t
+        let info := m!"Parsed have {t.subFrames}: type: {t.toType}, action: {t.action}"
+        return info
+    else if let some ⟨ tName, tInfo ⟩ := isTactic ["apply", "exact", "intro", "refine", "linarith_1"] i then
+      processTactic tName tInfo
+    else
+      let info := printInfo i true
+      let cs := (← children.mapM (parseTacticProof ctx lctx)) |>.toList
+      return MessageData.group $ info ++ MessageData.nest 2 (Format.line ++ MessageData.ofList cs)
+  | InfoTree.context ctx t => parseTacticProof ctx lctx t 
+  | _ => return m!"+++++++"
 
-  sorry
+-- Questions:
+-- 1) How to get a source code for the definiton?
 
-theorem exSeq (limit:
-  ∃ L, ∀ ε, ε > 0 → ∃ N, ∀ n, n ≥ N → dist (f n) L < ε): 3 < 4 := by
-  sorry
+partial def findChain (name : String) (types : PersistentHashMap String String) (frames : List Frame): List Frame := Id.run do
+  if name == solvedEmoji then
+    []
+  else
+    let type := types.findD name name
+    for frame in frames do
+      if frame.fromType == type then
+        return frame :: findChain frame.toType types frames
+    []
 
-/-
+elab "#buildTree" : command => do
+  let filename := "Example.lean"
+  let content ← IO.FS.readFile filename
+  let opts := Options.empty
+  let inputCtx := Parser.mkInputContext content filename
+  let (header, parserState, messages) ← Parser.parseHeader inputCtx
+  let (env, messages) ← processHeader header opts messages inputCtx 0
+  let env := env.setMainModule `Init
+  let mut commandState := Command.mkState env messages opts
 
+  let s ← IO.processCommands inputCtx parserState { commandState with infoState.enabled := true }
+  for msg in s.commandState.messages.toList do
+    IO.print (← msg.toString (includeEndPos := getPrintMessageEndPos opts))
+  let tree := s.commandState.infoState.trees[0]!
+  let (pp, ⟨ types, frames ⟩ ) ← (parseTacticProof none none tree).run ⟨ .empty, [] ⟩
+  let env := s.commandState.env
+  let expr := (env.find? `infinitude_of_primes).get!.toConstantVal.type
+  let type ← if let (.context ctx _) := tree then ctx.runMetaM {} (ppExpr expr) else return ()
+  let types := types.insert "top level" s!"{type}"
+  let fragments := findChain "h₂" types frames
+  for frag in fragments do
+    logInfo s!"{frag}"
+  logInfo "----------------"
+  for (name, type) in types.toList do
+    logInfo s!"{name} : {type}"
+  logInfo "----------------"
+  for frame in frames do
+    logInfo s!"{frame}"
+  logInfo pp
 
-
--- def list := [∃ L, ∀ ε, ∀ ε > 0, ∃ N, ∀ n, ∀ n ≥ N, dist (f n) L < ε]
--- def list2 := [∀ eps, ∀ ε > 0, ∃ δ, ∃ δ > 0, ∀ x y, ∀ dist x y < δ, dist (f x) (f y) < ε]
-
-theorem ex (limit:∀ ε, ε > 0 → ∃ δ, δ > 0 ∧
-(∀ x y, dist x y < δ → dist (f x) (f y) < ε)): 3 < 4 := by
-  have ε := 1
-  have hε : ε > 0 := by sorry
-  have ⟨ δ, ⟨ hδ, st ⟩ ⟩:= limit ε hε
-
-  sorry
--/
-
-structure GetPpContextParams where
-  pos : Lsp.Position
-  deriving FromJson, ToJson
-
-open Server RequestM in
-@[server_rpc_method]
-def getPpContext (params : GetPpContextParams): RequestM (RequestTask String) := do
-  withWaitFindSnapAtPos params.pos fun _ => do
-    pure "Hello from custom function"
-
-@[widget]
-def ppWidget: UserWidgetDefinition := {
-  name := "Paper proof"
-  javascript:= include_str "widget" / "dist" / "paperProof.js"
-}
-
-def test (x : ℕ):  ℕ :=
-  sorry
-
--- Check widget wiring
-#widget ppWidget .null
+#buildTree
