Example.lean
@@ -1,0 +1,27 @@
+import Mathlib.Data.Nat.Prime
+import Mathlib.Tactic.LibrarySearch
+import Mathlib.Tactic.Linarith
+ 
+theorem infinitude_of_primes : ∀ N, ∃ p, p ≥ N ∧ Nat.Prime p := by
+  intro N
+
+  let M := Nat.factorial N + 1
+  let p := Nat.minFac M
+
+  have pp : Nat.Prime p := by {
+    apply Nat.minFac_prime
+    have fac_pos: 0 < Nat.factorial N := Nat.factorial_pos N
+    linarith
+  }
+  have ppos: p ≥ N := by {
+    apply by_contradiction
+    intro pln
+    have h₁ : p ∣ Nat.factorial N := by  {
+      refine pp.dvd_factorial.mpr ?_
+      exact le_of_not_ge pln
+    }
+    have h₂ : p ∣ Nat.factorial N + 1 := Nat.minFac_dvd M
+    have h : p ∣ 1 := (Nat.dvd_add_right h₁).mp $ h₂
+    exact Nat.Prime.not_dvd_one pp h
+  }
+  exact ⟨ p, ppos, pp ⟩
